chore: broken?

RISCV/SailPure.lean
@@ -85,7 +85,7 @@ def remw (is_unsigned : Bool) (rs2_val : BitVec 64) (rs1_val : BitVec 64) : BitV
   let rem := if ((rs2_int == 0) : Bool) then rs1_int else Int.tmod rs1_int rs2_int
   sign_extend (m := ((2 ^i 3) *i 8)) (to_bits_truncate (l := 32) rem)
 
-def execute_MULW_pure64 (rs2_val : (BitVec 64)) (rs1_val : (BitVec 64)) : BitVec 64 :=
+def mulw (rs2_val : (BitVec 64)) (rs1_val : (BitVec 64)) : BitVec 64 :=
   let rs1_val32 := (Sail.BitVec.extractLsb rs1_val 31 0)
   let rs2_val32 := (Sail.BitVec.extractLsb rs2_val 31 0)
   let rs1_int : Int := (BitVec.toInt rs1_val32)
@@ -94,7 +94,7 @@ def execute_MULW_pure64 (rs2_val : (BitVec 64)) (rs1_val : (BitVec 64)) : BitVec
   let result : xlenbits := (sign_extend (m := ((2 ^i 3) *i 8)) result32)
   result
 
-def execute_MUL_pure64 (mul_op : mul_op) (rs2_val : (BitVec 64)) (rs1_val : (BitVec 64)) : BitVec 64 :=
+def mul (mul_op : mul_op) (rs2_val : (BitVec 64)) (rs1_val : (BitVec 64)) : BitVec 64 :=
   let rs1_int : Int := if mul_op.signed_rs1 then BitVec.toInt rs1_val else BitVec.toNat rs1_val
   let rs2_int : Int := if mul_op.signed_rs2 then BitVec.toInt rs2_val else BitVec.toNat rs2_val
   let result_wide := to_bits (l := 2 *i LeanRV64D.Functions.xlen) (rs1_int *i rs2_int)
